Using well formed judgements in poly proof

proof/Poly/Exp.v
@@ -14,124 +14,31 @@ Inductive exp : Type :=
 Hint Constructors exp.
 
 
-(* Closedness under type environment ********************************)
+(* Well Formedness **************************************************)
 
-(* Exp is val closed under a type environment of a given length *)
-Inductive coversXX : nat -> exp -> Prop :=
- | CoversXX_var
-   :  forall n i
-   ,  n > i
-   -> coversXX n (XVar i)
-
- | CoversXX_LAM
-   :  forall n x
-   ,  coversXX n x
-   -> coversXX n (XLAM x)
-
- | CoversXX_APP 
-   :  forall n x t
-   ,  coversXX n x
-   -> coversXX n (XAPP x t)
-
- | CoversXX_lam
-   :  forall n t x
-   ,  coversXX (S n) x
-   -> coversXX n (XLam t x)
-
- | CoversXX_app
-   :  forall n x1 x2
-   ,  coversXX n x1 -> coversXX n x2
-   -> coversXX n (XApp x1 x2).
-Hint Constructors coversXX.
+(* Exp is closed under the given environments *)
+Fixpoint wfX (kenv: env ki) (tenv: env ty) (xx: exp) : Prop := 
+ match xx with 
+ | XVar i     => exists t, get tenv i = Some t
+ | XLAM x     => wfX (kenv :> KStar) tenv x
+ | XAPP x t   => wfX kenv tenv x  /\ wfT kenv t
+ | XLam t x   => wfT kenv t       /\ wfX kenv (tenv :> t) x
+ | XApp x1 x2 => wfX kenv tenv x1 /\ wfX kenv tenv x2
+ end.
+Hint Unfold wfX.
 
 
-(* Exp is val closed under the given type environment *)
-Inductive closedUnderXX : tyenv -> exp -> Prop :=
-  |  ClosedUnderXX 
-     :  forall tenv x
-     ,  coversXX (length tenv) x
-     -> closedUnderXX tenv x.
-Hint Constructors closedUnderXX.
+(* Closed expressions are well formed under empty environments *)
+Definition closedX (xx: exp) : Prop
+ := wfX Empty Empty xx.
+Hint Unfold closedX.
 
 
-(* Exp is val closed under the empty type environment *)
-Inductive closedXX : exp -> Prop :=
- |  ClosedXX
-    :  forall x
-    ,  coversXX 0 x
-    -> closedXX x.
-Hint Constructors closedXX.
-
-
-(* Closedness under kind environment ********************************)
-
-(* Exp is type closed under a kind environment of a given length *)
-Inductive coversTX : nat -> exp -> Prop :=
- | CoversTX_var
-   :  forall n i
-   ,  coversTX n (XVar i)
-
- | CoversTX_LAM
-   :  forall n x
-   ,  coversTX (S n) x
-   -> coversTX n (XLAM x)
-
- | CoversTX_APP 
-   :  forall n x t
-   ,  coversTX n x
-   -> coversTT n t
-   -> coversTX n (XAPP x t)
-
- | CoversTX_lam
-   :  forall n t x
-   ,  coversTX n x
-   -> coversTX n (XLam t x)
-
- | CoversTX_app
-   :  forall n x1 x2
-   ,  coversTX n x1 -> coversTX n x2
-   -> coversTX n (XApp x1 x2).
-Hint Constructors coversTX.
-
-
-(* Exp is type closed under the given kind environment *)
-Inductive closedUnderTX : kienv -> exp -> Prop :=
-  |  ClosedUnderTX 
-     :  forall kenv x
-     ,  coversTX (length kenv) x
-     -> closedUnderTX kenv x.
-Hint Constructors closedUnderTX.
-
-
-(* Exp is type closed under the empty kind environment *)
-Inductive closedTX : exp -> Prop :=
- |  ClosedTX
-    :  forall x
-    ,  coversTX 0 x
-    -> closedTX x.
-Hint Constructors closedTX.
-
-
-(* Lemmas ***********************************************************)
-Lemma coversXX_succ
- :  forall n x
- ,  coversXX n     x
- -> coversXX (S n) x.
-Proof.
- intros. gen n.
- induction x; intros; inverts H; auto.
-Qed.
-Hint Resolve coversTT_succ.
-
-
-Lemma coversTX_succ
- :  forall n x
- ,  coversTX n     x
- -> coversTX (S n) x.
-Proof.
- intros. gen n.
- induction x; intros; inverts H; auto.
-Qed.
-Hint Resolve coversTX_succ.
+(* Values are closed expressions that cannot be reduced further *)
+Inductive value : exp -> Prop :=
+ | Value_lam 
+   : forall t x
+   , closedX (XLam t x) -> value (XLam t x).
+Hint Constructors value.
 
 
